\documentclass{article}

\usepackage{amsmath}

\begin{document}
\begin{enumerate}
	\item \begin{flalign*}
		              & \lim_{n \to + \infty}
		      \left[
			      \frac{ 1 }{ n }
			      \left(
			      \sqrt{\frac{ 1 }{ n } } +
			      \sqrt{\frac{ 2 }{ n } } +
			      \dots
			      \sqrt{\frac{ n }{ n } }
			      \right)
		      \right] &                       \\
	      \end{flalign*}

	\item \begin{flalign*}
		       & f(x) = \int_{\pi}^{x} \sin \left(\sqrt{s^2 + 4} \right) ds                               & \\
		       & u = \sqrt{s^2 + 4}                                                                       & \\
		       & u^2 = s^2 + 4                                                                            & \\
		       & 2u du = 2s ds                                                                            & \\
		       & u du = s ds                                                                              & \\
		       & ds = \frac{ u }{ s } du                                                                  & \\
		       & f(x) = \frac{ 1 }{ s } \int_{\sqrt{\pi^2 + 4}}^{\sqrt{x^2 + 4}} \frac{ \sin(u) }{ u } du & \\
	      \end{flalign*}

	\item \begin{enumerate}
		      \item \begin{flalign*}
			             & \frac{ dy }{ dx }                                                                                                       & \\
			             & e^{2x + 3y} = x^2 - \ln(xy^3)                                                                                           & \\
			             & \frac{ d }{ dx } \left(e^{2x + 3y}\right) = \frac{ d }{ dx } \left(x^2 - \ln(xy^3)\right)                               & \\
			             & e^{2x + 3y} \left(2 + 3 \frac{ dy }{ dx }\right)= 2x - \frac{ 1 }{ xy^3 } \left(y^3 + 3xy^2 \frac{ dy }{ dx } \right)   & \\
			             & 2 e^{2x + 3y} + 3 \left(e^{2x + 3y}\right) \frac{ dy }{ dx } = 2x - \frac{ 1 }{ x } + \frac{ 3 }{ y } \frac{ dy }{ dx } & \\
			             & 3 \left(e^{2x + 3y}\right) \frac{ dy }{ dx  } - \frac{ 3 }{ y } \frac{ dy }{ dx } = 2x - \frac{ 1 }{ x } - 2e^{2x + 3y} & \\
			             & \frac{ dy }{ dx } \left( 3(e^{2x + 3y}) - \frac{ 3 }{ y } \right) = 2x - \frac{ 1 }{ x } - 2e^{2x + 3y}                 & \\
		            \end{flalign*}

	      \end{enumerate}

	\item \begin{flalign*}
		       & f(x) = x^2                                             & \\
		       & g(x) = -x^2 + 8                                        & \\
		       & x^2 = -x^2 + 8 \implies x = \pm 2 \implies -2 < x < 2  & \\
		       & y = x^2 \implies x = \sqrt{y} = f(y)                   & \\
		       & y = -x^2 + 8 \implies x = \sqrt{8 - y} = g(y)          & \\
		       & V = \pi \int_{-2}^{2} [f(y)^2 - g(y)^2]dy              & \\
		       & V = \pi \int_{-2}^{2} (y - 8 + y) dy                   & \\
		       & V = \pi \int_{-2}^{2} (2y - 8) dy                      & \\
		       & V = y^2 \bigg\rvert_{-2}^{2} - 8y \bigg\rvert_{-2}^{2} & \\
		       & V = 2^2 - (-2)^2 - 8( 2 - (-2) )                       & \\
		       & V = -32\pi                                             & \\
		       &                                                        & \\
		       & V = \pi \int_{-2}^{2} (8 - y - y) dy                   & \\
		       & V = \pi \int_{-2}^{2} (8 - 2y) dy                      & \\
		       & V = 32 \pi                                             & \\
	      \end{flalign*}

	\item \begin{flalign*}
		       & \int_{-1}^{1} \arctan(x)                                                    & \\
		       &                                                                             & \\
		       & \int u dv = uv - \int v du                                                  & \\
		       & u = \arctan(x)                                                              & \\
		       & du = \frac{ 1 }{ x^2 + 1 } dx                                               & \\
		       & dv = dx                                                                     & \\
		       & v = x                                                                       & \\
		       &                                                                             & \\
		       & x \arctan(x) - \int_{-1}^{1} x \frac{ 1 }{ x^2 + 1 } dx                     & \\
		       & u = x^2 + 1                                                                 & \\
		       & du = 2x dx                                                                  & \\
		       & \frac{ du }{ 2 } = x dx                                                     & \\
		       & \int_{-1}^{1} \frac{ 1 }{ u } du = \ln|u| = \ln|1 + x^2|                    & \\
		       & \int_{-1}^{1} x \frac{ 1 }{ x^2 + 1 } dx = \frac{ \ln|1 + x^2| }{ 2 }       & \\
		       & \left(x \arctan(x) - \frac{ \ln|1 + x^2| }{ 2 }\right) \bigg\rvert_{-1}^{1} & \\
		       & \arctan(-1) - \frac{ \ln(2) }{ 2 } - \arctan(1) + \frac{ \ln(2) }{ 2 }      & \\
		       & \frac{ \pi }{ 4 } - \frac{ \pi }{ 4 }                                       & \\
		       & \int_{-1}^{1} \arctan(x) = 0                                                & \\
	      \end{flalign*}

	\item \begin{flalign*}
		       & x(x^2 - 1) = 0 \implies (x_1, x_2, x_3) = (-1, 0, 1)                                                                            & \\
		       & A = \int_{-1}^{0} (x^3 - x) dx + \int_{0}^{1} (x^3 - x) dx                                                                      & \\
		       & \int (x^3 - x) dx = \frac{ x^4 }{ 4 } - \frac{ x^2 }{ 2 }                                                                       & \\
		       &                                                                                                                                 & \\
		       & \left(\frac{ x^4 }{ 4 } - \frac{ x^2 }{ 2 } \right) \bigg\rvert_{-1}^{0}                                                        & \\
		       & = \frac{ 1 }{ 4 } - \frac{ 1 }{ 2 } = - \frac{ 1 }{ 4 }                                                                         & \\
		       &                                                                                                                                 & \\
		       & \left(\frac{ x^4 }{ 4 } - \frac{ x^2 }{ 2 } \right) \bigg\rvert_{0}^{1}                                                         & \\
		       & 0 - \left(- \frac{ 1 }{ 4 }\right) = \frac{ 1 }{ 4 }                                                                            & \\
		       & A = - \frac{ 1 }{ 4 } + \frac{ 1 }{ 4 } = 0                                                                                     & \\
		       &                                                                                                                                 & \\
		       & V = \pi \int_{-1}^{0} (x^3 - x)^2 dx + \pi \int_{0}^{1} (x^3 - x)^2 dx                                                          & \\
		       &                                                                                                                                 & \\
		       & \int (x^3 - x)^2 dx                                                                                                             & \\
		       & \int x^2(x^2 - 1)^2 dx                                                                                                          & \\
		       & \int x^2(x^4 - 2x^2 + 1) dx                                                                                                     & \\
		       & \int (x^6 - 2x^4 + x^2) dx                                                                                                      & \\
		       & \frac{ x^7 }{ 7 } - \frac{ 2x^5 }{ 5 } + \frac{ x^3 }{ 3 } \bigg\rvert_{-1}^{0}                                                 & \\
		       & - \frac{ 1 }{ 7 } + \frac{ 2 }{ 5 } - \frac{ 1 }{ 3 }                                                                           & \\
		       &                                                                                                                                 & \\
		       & \frac{ x^7 }{ 7 } - \frac{ 2x^5 }{ 5 } + \frac{ x^3 }{ 3 } \bigg\rvert_{0}^{1}                                                  & \\
		       & \frac{ 1 }{ 7 } - \frac{ 2 }{ 5 } + \frac{ 1 }{ 3 }                                                                             & \\
		       &                                                                                                                                 & \\
		       & V = - \frac{ \pi }{ 7 } + \frac{ 2 \pi }{ 5 } + \frac{ \pi }{ 3 } + \frac{ \pi }{ 7 } - \frac{ 2 \pi }{ 5 } + \frac{ \pi }{ 3 } & \\
		       & V = 0                                                                                                                           & \\
	      \end{flalign*}

	\item \begin{flalign*}
		       & \frac{ dC }{ dt } = 5 + 10te^{-t^2}                  & \\
		       & dC =  5 + 10te^{-t^2} dt                             & \\
		       & C = \int 5 + 10te^{-t^2} dt                          & \\
		       & C = 5t + 10 \int te^{-t^2} dt                        & \\
		       & u = -t^2                                             & \\
		       & du = -2t dt \implies - \frac{ 1 }{ 2 } du = t dt     & \\
		       & \int te^{-t^2} dt = - \frac{ 1 }{ 2 } \int e^u du    & \\
		       & = - \frac{ 1 }{ 2 } e^u = - \frac{ 1 }{ 2 } e^{-t^2} & \\
		       & C = 5t + 10 \left( -\frac{ 1 }{ 2 } e^{-t^2} \right) & \\
		       & C = 5t - 5e^{-t^2}                                   & \\
	      \end{flalign*}

\end{enumerate}
\end{document}
