\documentclass{article}

\usepackage{enumitem}
\usepackage{amsmath}

\begin{document}

\begin{enumerate}
	\item \begin{enumerate}[label=1.\arabic*]
		      \item \begin{flalign*}
			             & \lim_{x \to 2} ax^2 + 2x = \lim_{x \to 2} x^3 - ax & \\
			             & 4a + 4 = 8 - 2a                                    & \\
			             & a = \frac{ 2 }{ 3 }                                & \\
		            \end{flalign*}

		      \item \begin{flalign*}
			             & \lim_{x \to 2} \frac{ x^2 - 4 }{ x - 2 } = \lim_{x \to 2} ax^2 - bx + 3         & \\
			             & \lim_{x \to 2} \frac{ (x  + 2)(x - 2) }{ x - 2 } = \lim_{x \to 2} ax^2 - bx + 3 & \\
			             & \lim_{x \to 2} x + 2 = \lim_{x \to 2} ax^2 - bx + 3                             & \\
			             & 4 = 4a - 2b + 3                                                                 & \\
			             & 4a - 2b = 1                                                                     & \\
			             &                                                                                 & \\
			             & \lim_{x \to 3} ax^2 - bx + 3 = \lim_{x \to 3} 2x - a + b                        & \\
			             & 9a - 3b + 3 = 6 - a + b                                                         & \\
			             & 10a - 2b = 3                                                                    & \\
			             &                                                                                 & \\
			             & \begin{cases}
				               10a - 2b = 3 \\
				               4a - 2b = 1  \\
			               \end{cases}                                                                 &     \\
			             & 6a = 2                                                                          & \\
			             & a = \frac{ 1 }{ 3 }                                                             & \\
			             & \frac{ 4 }{ 3 } - 2b = 1                                                        & \\
			             & b = \frac{\frac{ 4 }{ 3 } - 1}{2}                                               & \\
			             & b = \frac{ 1 }{ 6 }                                                             & \\
		            \end{flalign*}

	      \end{enumerate}

	\item \begin{enumerate}[label=2.\arabic*]
		      \item \begin{flalign*}
			             & \lim_{x \to \infty} \left( 2 - \frac{ 1 }{ x } + \frac{ 4 }{ x^2 } \right) = 2 - 0 + 0 = 2 & \\
		            \end{flalign*}

		      \item \begin{flalign*}
			             & \lim_{x \to -\infty} \frac{ 4x^3 - 2x^2 + 1 }{ 3x^3 - 5 }                                                                                      & \\
			             & \lim_{x \to -\infty} \frac{ 4 - \frac{ 2 }{ x } + \frac{ 1 }{ x^3 } }{ 3 - \frac{ 5 }{ x^3 } } = \frac{ 4 - 0 + 0 }{ 3 - 0 } = \frac{ 4 }{ 3 } & \\
		            \end{flalign*}

		      \item \begin{flalign*}
			             & \lim_{x \to \infty} \frac{ x + 1 }{ x }             & \\
			             & \lim_{x \to \infty} 1 + \frac{ 1 }{ x } = 1 + 0 = 1 & \\
		            \end{flalign*}

		      \item \begin{flalign*}
			             & \lim_{x \to -\infty} \frac{ x + 1 }{ x } = -1 & \\
		            \end{flalign*}

		      \item \begin{flalign*}
			             & \lim_{x \to -\infty} \frac{ x^2 + x - 1 }{ 2x + 5 }                                    & \\
			             & \lim_{x \to -\infty} \frac{ x + 1 - \frac{ 1 }{ x } }{ 2 + \frac{ 5 }{ x } } = -\infty & \\
		            \end{flalign*}

		      \item \begin{flalign*}
			             & \lim_{x \to \infty} \frac{ x - 2 }{ \sqrt{2 + x} } & \\
		            \end{flalign*}

	      \end{enumerate}

	\item \begin{enumerate}[label=3.\arabic*]
		      \item \begin{flalign*}
			             & f(x) = \frac{ 1 }{ x^2 - 4 } & \\
		            \end{flalign*}

		      \item \begin{flalign*}
			             & f(x) = \frac{ 2x^2 }{ x^2 + 1 } & \\
		            \end{flalign*}

		      \item \begin{flalign*}
			             & f(x) = \frac{ x^2 + 3x + 2 }{ x^2 + 2x - 3 } & \\
		            \end{flalign*}

		      \item \begin{flalign*}
			             & \frac{ x^4 }{ x^2 - 16 } & \\
		            \end{flalign*}

	      \end{enumerate}
\end{enumerate}

\end{document}
