\documentclass{article}

\usepackage{amsmath}

\begin{document}
\begin{enumerate}
	\item
	      \begin{tabular}{ |c|c| }
		      x   & y    \\
		      \hline
		      1.3 & 3.2  \\
		      1.8 & 4.3  \\
		      2.6 & 0.5  \\
		      3.9 & -1.7 \\
		      \hline
	      \end{tabular}
	      \begin{flalign*}
		       & L_0 = \frac{ (x - x_1)(x - x_2)(x - x_3) }{ (x_0 - x_1)(x_0 - x_2)(x_0 - x_3) } & \\
		       & L_1 = \frac{ (x - x_0)(x - x_2)(x - x_3) }{ (x_1 - x_0)(x_1 - x_2)(x_1 - x_3) } & \\
		       & L_2 = \frac{ (x - x_0)(x - x_1)(x - x_3) }{ (x_2 - x_0)(x_2 - x_1)(x_2 - x_3) } & \\
		       & L_3 = \frac{ (x - x_0)(x - x_1)(x - x_2) }{ (x_3 - x_0)(x_3 - x_1)(x_3 - x_2) } & \\
		       & P_3(x) = y_0 L_0 + y_1 L_1 + y_2 L_2 + y_3 L_3                                  & \\
		       &                                                                                 & \\
		       & L_0 = \frac{ (x - 1.8)(x - 2.6)(x - 3.9) }{ (1.3 - 1.8)(1.3 - 2.6)(1.3 - 3.9) } & \\
		       & L_1 = \frac{ (x - 1.3)(x - 2.6)(x - 3.9) }{ (1.8 - 1.3)(1.8 - 2.6)(1.8 - 3.9) } & \\
		       & L_2 = \frac{ (x - 1.3)(x - 1.8)(x - 3.9) }{ (2.6 - 1.3)(2.6 - 1.8)(2.6 - 3.9) } & \\
		       & L_3 = \frac{ (x - 1.3)(x - 1.8)(x - 2.6) }{ (3.9 - 1.3)(3.9 - 1.8)(3.9 - 2.6) } & \\
		       & P_3(x) = 3.2 L_0 + 4.3 L_1 + 0.5 L_2 + (-1.7)L_3                                & \\
	      \end{flalign*}

\end{enumerate}
\end{document}
