\documentclass{article}

\usepackage{amsmath}
\usepackage{tikz}

\begin{document}
\begin{enumerate}
	\item
	\item \begin{flalign*}
		       & h(x) = x^3 - x^2 - x \text{ com } -2 \le x \le 2                                             & \\
		       & h'(x) = 3x^2 - 2x - 1                                                                        & \\
		       & 3x^2 - 2x - 1 = 0                                                                            & \\
		       & (x_1, x_2) = \left( 1, - \frac{ 1 }{ 3 } \right)                                             & \\
		       & h(1) = -1                                                                                    & \\
		       & h\left( - \frac{ 1 }{ 3 } \right) = - \frac{ 1 }{ 27 } - \frac{ 1 }{ 9 } + \frac{ 1 }{ 3 }   & \\
		       & h\left( - \frac{ 1 }{ 3 } \right) = - \frac{ 1 }{ 27 } - \frac{ 3 }{ 27 } + \frac{ 9 }{ 27 } & \\
		       & h\left( - \frac{ 1 }{ 3 } \right) = \frac{ 5 }{ 27 }                                         & \\
		       & h(-2) = -8 - 4 + 2 = -10                                                                     & \\
		       & h(2) = 8 - 4 - 2 = 2                                                                         & \\
		       & \text{Min} \implies -10                                                                      & \\
		       & \text{Max} \implies 2                                                                        & \\
	      \end{flalign*}

	\item
	      \begin{flalign*}
		       & p = A \times v                                         & \\
		       & \pi r^2 h = 1                                          & \\
		       & A = 2 \pi r^2 + 2 \pi r h                              & \\
		       &                                                        & \\
		       & h = \frac{ 1 }{ \pi r^2 }                              & \\
		       & A = 2 \pi r^2 + 2 \pi r \frac{ 1 }{ \pi r^2 }          & \\
		       & A = 2 \pi r^2 + \frac{ 2 }{ r }                        & \\
		       & A' = 4 \pi r - \frac{ 2 }{ r^2 }                       & \\
		       &                                                        & \\
		       & 4 \pi r - \frac{ 2 }{ r^2 } = 0                        & \\
		       & 4 \pi r^3 - 2 = 0                                      & \\
		       & r = \sqrt[3]{\frac{ 1 }{ 2 \pi } }                     & \\
		       & h = \frac{ 1 }{ \pi \sqrt[3]{\frac{ 1 }{ 4 \pi^2 } } } & \\
	      \end{flalign*}

	\item
	      \begin{flalign*}
		       & a + c = 3       & \\
		       & b = 3           & \\
		       & \text{Max}(abc) & \\
	      \end{flalign*}


	\item \begin{enumerate}
		      \item
		            \begin{flalign*}
			             & f(t) = t(100 - t) = 100t - t^2 & \\
			             & f'(t) = 100 - 2t               & \\
			             & 100 - 2t = 0 \implies t = 50   & \\
			             & f(50) = 50(100 - 50) = 2500    & \\
		            \end{flalign*}

		      \item
		            \begin{flalign*}
			             & f(40) = 2400 & \\
		            \end{flalign*}
	      \end{enumerate}


\end{enumerate}
\end{document}
