\documentclass{article}

\usepackage{amsmath}

\title{Lista 3 - Calculo I}
\author{}

\begin{document}
\maketitle

\begin{enumerate}
	\item
	\item
	\item
	\item
	\item
	\item
	\item
	\item
	\item
	\item \begin{flalign*}
		       & \frac{ d }{ dx } (3x^3 - 2x^2 + x - 100) & \\
		       & 9x^2 - 4x + 1                            & \\
	      \end{flalign*}

	\item
	      \begin{flalign*}
		       & \frac{ d }{ dx } \left( \frac{ 1 - x }{ x + 1 } \right)  & \\
		       & \frac{ (1 - x)' (x + 1) - (1 - x)(x + 1)' }{ (x + 1)^2 } & \\
		       & \frac{ 1 (x + 1) - (1 - x) (1) }{ (x + 1)^2 }            & \\
		       & \frac{ (x + 1) - (1 - x) }{ (x + 1)^2 }                  & \\
		       & \frac{ x + 1 - 1 + x }{ (x + 1)^2 }                      & \\
		       & \frac{ 2x }{ (x + 1)^2 }                                 & \\
	      \end{flalign*}

	\item
	      \begin{flalign*}
		       & f'(x) = \frac{ d }{ dx } \left( x^3 - 6x^2 + 9x - 1 \right) & \\
		       & f'(x) = 3x^2 - 12x + 9                                      & \\
		       & 3x^2 - 12x + 9 = 0                                          & \\
		       & x^2 - 4x + 3 = 0                                            & \\
		       & (x_1, x_2) = (1, 3)                                         & \\
	      \end{flalign*}

	\item
	      \begin{flalign*}
		       & L'(p) = \frac{ d }{ dx } \left( -p^3 + 7p^2 - 11p + 5 \right)  & \\
		       & L'(p) = -3p^2 + 14p - 11                                       & \\
		       & -3p^2 + 14p - 11 = 0                                           & \\
		       & 3p^2 - 14p + 11 = 0                                            & \\
		       & (x_1, x_2) = \frac{ 14 \pm \sqrt{196 - 12 \times 11} }{ 6 }    & \\
		       & (x_1, x_2) = \frac{ 14 \pm \sqrt{196 - 132} }{ 6 }             & \\
		       & (x_1, x_2) = \frac{ 14 \pm \sqrt{64} }{ 6 }                    & \\
		       & (x_1, x_2) = \frac{ 14 \pm 8 }{ 6 }                            & \\
		       & (x_1, x_2) = \left( \frac{ 22 }{ 6 } , \frac{ 6 }{ 6 } \right) & \\
		       & (x_1, x_2) = \left( \frac{ 11 }{ 3 } , 1 \right)               & \\
	      \end{flalign*}

	\item
	\item
	      \begin{flalign*}
		       & f'(x) = \frac{ d }{ dx } \left( \frac{ 1 }{ x } \right) & \\
		       & f'(x) = \frac{ 0 \times  x - 1 \times  1}{ x^2 }        & \\
		       & f'(x) = - \frac{1}{ x^2 }                               & \\
		       & f'(1) = - \frac{1}{ 1^2 } = -1                          & \\
	      \end{flalign*}

\end{enumerate}
\end{document}
