\documentclass{article}

\usepackage{amsmath}

\begin{document}
\begin{flalign*}
	 & y_{n + 1} = y_n + h f(x_n, y_n) & \\
	 & x_{n + 1} = x_n + h             & \\
\end{flalign*}

\begin{flalign*}
	 & \begin{cases}
		   2y - 2 = xy' \Rightarrow y' = \frac{ 2y - 2 }{ x } \\
		   y(1) = 3                                           \\
	   \end{cases}        &             \\
	 & (x_0, y_0) = (1, 3)                                          & \\
	 & h = 0.5                                                      & \\
	 & n = 2                                                        & \\
	 & y_1 = y_0 + 0.5 f(x_0, y_0)                                  & \\
	 & y_1 = 3 + 0.5 \left( \frac{ 2 \cdot 3 - 2 }{ 1 } \right) = 5 & \\
	 & x_1 = 1 + 0.5 = 1.5                                          & \\
	 &                                                              & \\
	 & y_2 = 5 + 0.5 \left( \frac{ 2 \cdot 5 - 2 }{ 1.5 } \right)   & \\
	 & y_2 = y(2) = \frac{ 11.5 }{ 1.5 } = \frac{ 23 }{ 3 }         & \\
\end{flalign*}
\end{document}
