\documentclass{article}

\usepackage{amsmath}

\author{Carlos Eduardo Carvalho de Souza}
\title{Calculo I - P1 2023.1}
\begin{document}
\maketitle

\begin{enumerate}
	\item d
	\item
	\item a
	\item a
	\item a
	\item a
	      \begin{flalign*}
		       & f'(x) = \frac{ d }{ dx } \left( 3x^3 - 2x + 1 \right) & \\
		       & f'(x) = 9x^2 - 2                                      & \\
		       & f'(-1) = 9 (-1)^2 - 2 = 9 - 2 = 7                       \\
		       & y = 7x + b                                            & \\
		       & 0 = 7 (-1) + b \iff b = 7                             & \\
		       & y = 7x + 7                                            & \\
	      \end{flalign*}

	\item d
	      \begin{flalign*}
		       & -2 + \frac{ 1 }{ (-2)^2 } = -2 + \frac{ 1 }{ 4 } < 0 & \\
		       & 2 + \frac{ 1 }{ 4 } > 0                              & \\
	      \end{flalign*}

	\item a
	      \begin{flalign*}
		       & L'(p) = \frac{ d }{ dx } \left( -p^2 + 5p + 2 \right) & \\
		       & L'(p) = -2p + 5                                       & \\
		       & -2p + 5 = 0 \implies 2p = 5 \implies p = 2.5          & \\
	      \end{flalign*}

	\item d
	\item c
	\item
	      \begin{flalign*}
		       & f(1) = 1    & \\
		       & g(1) = 0    & \\
		       & f'(x) = 2x  & \\
		       & g'(x) = -2x & \\
	      \end{flalign*}

	\item b
	\item a
	      \begin{flalign*}
		       & L = ax + b                                                & \\
		       & y' = 3x^2                                                 & \\
		       & L = 3x + b                                                & \\
		       & 8 = 3 + b \iff b = 5                                      & \\
		       & L = 3x + 5                                                & \\
		       & L(0) = 5                                                  & \\
		       & L(x) = 0 \implies x = - \frac{ 5 }{ 3 }                   & \\
		       & \frac{ 5 \times \frac{ 5 }{ 3 } }{ 2 } = \frac{ 25 }{ 6 } & \\
	      \end{flalign*}

	\item a
	      \begin{flalign*}
		       & h(x) = f(x)g(x)                  & \\
		       & h(1) = f(1)g(1)                  & \\
		       & 24 = f(1) \times 6 \iff f(1) = 4 & \\
		       &                                  & \\
		       & h'(x) = f'(x)g(x) + f(x)g'(x)    & \\
		       & h'(1) = f'(1)g(1) + f(1)g'(1)    & \\
		       & 20 = 2 \times 6 + 4g'(1)         & \\
		       & 20 = 12 + 4g'(1)                 & \\
		       & 8 = 4g'(1)                       & \\
		       & g'(1) = 2                        & \\
	      \end{flalign*}

	\item a
	      \begin{flalign*}
		       & f'(x) = \frac{ d }{ dx } \left( \frac{ x^2 - 2x + 3 }{ x - 1 } \right)                                          & \\
		       & f'(x) = \frac{ \frac{ d }{ dx } (x^2 - 2x + 3) (x - 1) - (x^2 - 2x + 3) \frac{ d }{ dx } (x - 1) }{ (x - 1)^2 } & \\
		       & f'(x) = \frac{ (2x - 2)(x - 1) - (x^2 - 2x + 3) }{ (x - 1)^2 }                                                  & \\
		       & f'(x) = \frac{ 2x^2 - 2x - 2x + 2 - x^2 + 2x - 3 }{ (x - 1)^2 }                                                 & \\
		       & f'(x) = \frac{ x^2 - 2x - 1 }{ (x - 1)^2 }                                                                      & \\
	      \end{flalign*}


\end{enumerate}
\end{document}
